src/QueryStructure/Automation/AutoDB.v
@@ -95,56 +95,51 @@ Ltac FullySharpenEachMethod delegateSigs delegateSpecs cRep' cAbsR' :=
   end; simpl; repeat split.
 
 Definition Build_IndexedQueryStructure_Impl_Sigs
-           {indices : list NamedSchema}
-           (Index : ilist (fun ns : NamedSchema => SearchUpdateTerms (schemaHeading (relSchema ns))) indices)
-           (idx : @BoundedString (map relName indices))
+           {n}
+           {indices : Vector.t RawSchema n}
+           (Index : ilist2 (B := fun sch => SearchUpdateTerms (rawSchemaHeading sch)) indices)
+           (idx : Fin.t _)
 : ADTSig :=
-  BagSig (@Tuple (schemaHeading (relSchema (nth_Bounded relName indices idx))))
-         (BagSearchTermType (ith_Bounded _ Index idx))
-         (BagUpdateTermType (ith_Bounded _ Index idx)).
+  BagSig (@RawTuple (rawSchemaHeading (Vector.nth indices idx)))
+         (BagSearchTermType (ith2 Index idx))
+         (BagUpdateTermType (ith2 Index idx)).
 
 Definition Build_IndexedQueryStructure_Impl_Specs
-           {indices : list NamedSchema}
-           (Index : ilist (fun ns : NamedSchema => SearchUpdateTerms (schemaHeading (relSchema ns))) indices)
-           (idx : @BoundedString (map relName indices))
-: ADT (@Build_IndexedQueryStructure_Impl_Sigs indices Index idx) :=
-  @BagSpec (@Tuple (schemaHeading (relSchema (nth_Bounded relName indices idx))))
-           (BagSearchTermType (ith_Bounded _ Index idx))
-           (BagUpdateTermType (ith_Bounded _ Index idx))
-           (BagMatchSearchTerm (ith_Bounded _ Index idx))
-           (BagApplyUpdateTerm (ith_Bounded _ Index idx)).
-
+           {n}
+           {indices : Vector.t RawSchema n}
+           (Index : ilist2 (B := fun sch => SearchUpdateTerms (rawSchemaHeading sch)) indices)
+           (idx : Fin.t _)
+: ADT (@Build_IndexedQueryStructure_Impl_Sigs n indices Index idx) :=
+  @BagSpec (@RawTuple (rawSchemaHeading (Vector.nth indices idx)))
+           (BagSearchTermType (ith2 Index idx))
+           (BagUpdateTermType (ith2 Index idx))
+           (BagMatchSearchTerm (ith2 Index idx))
+           (BagApplyUpdateTerm (ith2 Index idx)).
 Definition
   Build_IndexedQueryStructure_Impl_cRep
-  (indices : list NamedSchema)
-  (Index : ilist
-             (fun ns : NamedSchema =>
-                SearchUpdateTerms (schemaHeading (relSchema ns))) indices)
-  (DelegateReps : @BoundedString (map relName indices) -> Type)
+  {n}
+  {indices : Vector.t RawSchema n}
+  (Index : ilist2 (B := fun sch => SearchUpdateTerms (rawSchemaHeading sch)) indices)
+  (DelegateReps : Fin.t n -> Type)
 : Type :=
   Iterate_Dep_Type_BoundedIndex DelegateReps.
 
 Definition
   GetIndexedQueryStructureRelation
-  {indices : list NamedSchema}
-  {Index : ilist
-             (fun ns : NamedSchema =>
-                SearchUpdateTerms (schemaHeading (relSchema ns))) indices}
-  {DelegateReps : @BoundedString (map relName indices) -> Type}
+  {n}
+  {indices : Vector.t RawSchema n}
+  {Index : ilist2 (B := fun sch => SearchUpdateTerms (rawSchemaHeading sch)) indices}
+  {DelegateReps : Fin.t n -> Type}
   (r_n : Build_IndexedQueryStructure_Impl_cRep Index DelegateReps)
   idx
 : DelegateReps idx :=
-  match idx with
-      {|bindex := idx;
-        indexb := {| ibound := n;
-                     boundi := nth_n |} |} =>
-      Lookup_Iterate_Dep_Type string_dec DelegateReps r_n n nth_n
-  end.
+  Lookup_Iterate_Dep_Type DelegateReps r_n idx.
 
 Definition Build_IndexedQueryStructure_Impl_AbsR
-           {qs_schema : QueryStructureSchema}
-           (Index : ilist (fun ns : NamedSchema => SearchUpdateTerms (schemaHeading (relSchema ns))) (qschemaSchemas qs_schema) )
-           (DelegateReps : @BoundedString (map relName (qschemaSchemas qs_schema)) -> Type)
+           {qs_schema : RawQueryStructureSchema}
+           (Index : ilist2 (B := fun sch => SearchUpdateTerms (rawSchemaHeading sch))
+                           (qschemaSchemas qs_schema))
+           (DelegateReps : Fin.t _ -> Type)
            (DelegateImpls : forall idx,
                               ComputationalADT.pcADT (Build_IndexedQueryStructure_Impl_Sigs Index idx) (DelegateReps idx))
            (ValidImpls
@@ -154,14 +149,15 @@ Definition Build_IndexedQueryStructure_Impl_AbsR
            (r_o : IndexedQueryStructure qs_schema Index)
            (r_n : Build_IndexedQueryStructure_Impl_cRep Index DelegateReps)
 : Prop :=
-  forall idx : @BoundedString (map relName (qschemaSchemas qs_schema)),
+  forall idx : Fin.t _,
     AbsR (ValidImpls idx)
          (GetIndexedRelation r_o idx) (GetIndexedQueryStructureRelation r_n idx).
 
 Definition CallBagImplMethod
-           {schemas : list NamedSchema}
-           (Index : ilist (fun ns : NamedSchema => SearchUpdateTerms (schemaHeading (relSchema ns))) (schemas))
-           (DelegateReps : @BoundedString (map relName schemas) -> Type)
+           {n}
+           {schemas : Vector.t RawSchema n}
+           (Index : ilist2 (B := fun sch => SearchUpdateTerms (rawSchemaHeading sch)) schemas)
+           (DelegateReps : Fin.t _ -> Type)
            (DelegateImpls : forall idx,
                               ComputationalADT.pcADT (Build_IndexedQueryStructure_Impl_Sigs Index idx) (DelegateReps idx))
            idx midx
@@ -169,27 +165,29 @@ Definition CallBagImplMethod
   ComputationalADT.pcMethods (DelegateImpls idx) midx (GetIndexedQueryStructureRelation r_n idx).
 
 Definition CallBagImplConstructor
-           {schemas : list NamedSchema}
-           (Index : ilist (fun ns : NamedSchema => SearchUpdateTerms (schemaHeading (relSchema ns))) schemas )
-           (DelegateReps : @BoundedString (map relName schemas) -> Type)
+           {n}
+           {schemas : Vector.t RawSchema n}
+           (Index : ilist2 (B := fun sch => SearchUpdateTerms (rawSchemaHeading sch)) schemas)
+           (DelegateReps : Fin.t _ -> Type)
            (DelegateImpls : forall idx,
                               ComputationalADT.pcADT (Build_IndexedQueryStructure_Impl_Sigs Index idx) (DelegateReps idx))
            idx cidx :=
   ComputationalADT.pcConstructors (DelegateImpls idx) cidx.
 
 Lemma refine_BagImplConstructor
-      {schemas : list NamedSchema}
-      (Index : ilist (fun ns : NamedSchema => SearchUpdateTerms (schemaHeading (relSchema ns))) schemas )
-      (DelegateReps : @BoundedString (map relName schemas) -> Type)
-      (DelegateImpls : forall idx,
-                         ComputationalADT.pcADT (Build_IndexedQueryStructure_Impl_Sigs Index idx) (DelegateReps idx))
-      (ValidImpls
-       : forall idx,
-           refineADT (Build_IndexedQueryStructure_Impl_Specs Index idx)
-                     (ComputationalADT.LiftcADT (existT _ _ (DelegateImpls idx))))
-:  forall (ridx : BoundedIndex (map relName schemas)) cidx d,
+      {n}
+           {schemas : Vector.t RawSchema n}
+           (Index : ilist2 (B := fun sch => SearchUpdateTerms (rawSchemaHeading sch)) schemas)
+           (DelegateReps : Fin.t _ -> Type)
+           (DelegateImpls : forall idx,
+               ComputationalADT.pcADT (Build_IndexedQueryStructure_Impl_Sigs Index idx) (DelegateReps idx))
+           (ValidImpls
+            : forall idx,
+               refineADT (Build_IndexedQueryStructure_Impl_Specs Index idx)
+                          (ComputationalADT.LiftcADT (existT _ _ (DelegateImpls idx))))
+:  forall (ridx : Fin.t _) cidx d,
    exists r_o' ,
-     refine (@CallBagConstructor _ (bindex ridx) (ith_Bounded relName Index ridx) cidx d)
+     refine (@CallBagConstructor _ (ith2 Index ridx) cidx d)
             (ret r_o') /\
      AbsR (ValidImpls ridx) r_o' (CallBagImplConstructor DelegateReps DelegateImpls cidx d).
 Proof.
@@ -201,22 +199,22 @@ Proof.
   split; simpl.
   - intros v' Comp_v;  computes_to_inv; subst.
     generalize d v' H; clear.
-    eapply (fun P H => Iterate_Dep_Type_BoundedString_equiv_1 P H cidx).
+    eapply (fun P H => Lookup_Iterate_Dep_Type P H cidx).
     simpl; intuition.
   - eapply H'.
 Qed.
 
 Lemma refine_BagImplMethods
-      {qs_schema : QueryStructureSchema}
-      (indices := qschemaSchemas qs_schema)
-      (Index : ilist (fun ns : NamedSchema => SearchUpdateTerms (schemaHeading (relSchema ns))) (qschemaSchemas qs_schema) )
-      (DelegateReps : @BoundedString (map relName (qschemaSchemas qs_schema)) -> Type)
+      {qs_schema : RawQueryStructureSchema}
+      (schemas := qschemaSchemas qs_schema)
+      (Index : ilist2 (B := fun sch => SearchUpdateTerms (rawSchemaHeading sch)) schemas)
+      (DelegateReps : Fin.t _ -> Type)
       (DelegateImpls : forall idx,
-                         ComputationalADT.pcADT (Build_IndexedQueryStructure_Impl_Sigs Index idx) (DelegateReps idx))
+          ComputationalADT.pcADT (Build_IndexedQueryStructure_Impl_Sigs Index idx) (DelegateReps idx))
       (ValidImpls
        : forall idx,
-           refineADT (Build_IndexedQueryStructure_Impl_Specs Index idx)
-                     (ComputationalADT.LiftcADT (existT _ _ (DelegateImpls idx))))
+          refineADT (Build_IndexedQueryStructure_Impl_Specs Index idx)
+                    (ComputationalADT.LiftcADT (existT _ _ (DelegateImpls idx))))
 :  forall (r_o : IndexedQueryStructure qs_schema Index)
           (r_n : Build_IndexedQueryStructure_Impl_cRep Index DelegateReps)
           ridx,
@@ -245,37 +243,38 @@ Proof.
     intros v' Comp_v; simpl in *;  computes_to_inv; subst.
     destruct v; simpl @fst in *; simpl @snd in *.
     generalize d i m H H0; clear.
-    eapply (fun P H => Iterate_Dep_Type_BoundedString_equiv_1 P H midx).
+    eapply (fun P H => Lookup_Iterate_Dep_Type P H midx).
     simpl; intuition.
     eassumption.
   - unfold ComputationalADT.cMethods in *; simpl in *; rewrite <- H0''; eapply H0'.
 Qed.
 
 Definition Initialize_IndexedQueryStructureImpls'
+           {n}
            {schemas}
-           Index
-           (DelegateReps : @BoundedString (map relName schemas) -> Type)
+           (Index : ilist2 (n := n) (B := fun sch => SearchUpdateTerms (rawSchemaHeading sch)) schemas)
+           (DelegateReps : Fin.t _ -> Type)
            (DelegateImpls : forall idx,
                               ComputationalADT.pcADT (Build_IndexedQueryStructure_Impl_Sigs Index idx) (DelegateReps idx))
-: @Build_IndexedQueryStructure_Impl_cRep _ Index DelegateReps :=
-  Iterate_Dep_Type_equiv'
-    string_dec
-    (fun idx : @BoundedString (map relName schemas) =>
-       DelegateReps idx)
-    (fun idx : @BoundedString (map relName schemas) =>
-       CallBagImplConstructor DelegateReps DelegateImpls BagEmpty ()).
+  : @Build_IndexedQueryStructure_Impl_cRep _ _ Index DelegateReps :=
+  Iterate_Dep_Type_equiv''
+    DelegateReps
+    (fun idx  =>
+       CallBagImplConstructor DelegateReps DelegateImpls BagEmpty () ).
 
 Lemma Initialize_IndexedQueryStructureImpls_AbsR
-      {qs_schema : QueryStructureSchema}
-: forall (Index : ilist (fun ns : NamedSchema => SearchUpdateTerms (schemaHeading (relSchema ns))) (qschemaSchemas qs_schema) )
-         (DelegateReps : @BoundedString (map relName (qschemaSchemas qs_schema)) -> Type)
-         (DelegateImpls : forall idx,
-                            ComputationalADT.pcADT (Build_IndexedQueryStructure_Impl_Sigs Index idx) (DelegateReps idx))
-         (ValidImpls
-          : forall idx,
-              refineADT (Build_IndexedQueryStructure_Impl_Specs Index idx)
-                        (ComputationalADT.LiftcADT (existT _ _ (DelegateImpls idx)))),
-    refine (r_o <- @Initialize_IndexedQueryStructure _ Index;
+      {qs_schema : RawQueryStructureSchema}
+  : forall
+    (Index : ilist2 (B := fun sch => SearchUpdateTerms (rawSchemaHeading sch))
+                    (qschemaSchemas qs_schema))
+    (DelegateReps : Fin.t _ -> Type)
+    (DelegateImpls : forall idx,
+        ComputationalADT.pcADT (Build_IndexedQueryStructure_Impl_Sigs Index idx) (DelegateReps idx))
+    (ValidImpls
+     : forall idx,
+        refineADT (Build_IndexedQueryStructure_Impl_Specs Index idx)
+                  (ComputationalADT.LiftcADT (existT _ _ (DelegateImpls idx)))),
+    refine (r_o <- @Initialize_IndexedQueryStructure _ _ Index;
            {r_n | Build_IndexedQueryStructure_Impl_AbsR DelegateReps DelegateImpls ValidImpls r_o r_n})
            (ret (Initialize_IndexedQueryStructureImpls' DelegateReps DelegateImpls)).
 Proof.
@@ -283,71 +282,48 @@ Proof.
   unfold Build_IndexedQueryStructure_Impl_AbsR, GetIndexedRelation.
   simpl; clear qschemaConstraints.
   induction qschemaSchemas; intros;
-  pose proof (ilist_invert Index) as H'; simpl in H'; subst.
+  pose proof (ilist2_invert _ Index) as H'; simpl in H'; subst.
   - simpl; simplify with monad laws.
     computes_to_econstructor;  computes_to_inv; subst.
-    eapply (fun P H => Iterate_Dep_Type_BoundedString_equiv_1 P H); simpl.
+    eapply (Lookup_Iterate_Dep_Type); simpl.
     econstructor.
   - destruct H' as [idx' [Index' Index_eq]]; subst.
     simpl; simplify with monad laws.
     pose proof (IHqschemaSchemas
                   Index'
-                  (fun idx : @BoundedString (map relName qschemaSchemas) =>
-                     (DelegateReps {|bindex := bindex idx;
-                                     indexb := @IndexBound_tail _ _ _ _ (indexb idx) |}))
-                  (fun idx : @BoundedString (map relName qschemaSchemas) =>
-                     (DelegateImpls {|bindex := bindex idx;
-                                     indexb := @IndexBound_tail _ _ _ _ (indexb idx) |}))
-                  (fun idx : @BoundedString (map relName qschemaSchemas)=>
-                     (ValidImpls {|bindex := bindex idx;
-                                   indexb := @IndexBound_tail _ _ _ _ (indexb idx) |}))
+                  (fun idx => DelegateReps (Fin.FS idx))
+                  (fun idx => DelegateImpls (Fin.FS idx))
+                  (fun idx => ValidImpls (Fin.FS idx))
                _ (ReturnComputes _)).
     unfold refine; intros;  computes_to_inv; subst.
     computes_to_econstructor; eauto.
     computes_to_econstructor.
     intros.
     pose proof (fun d => @refine_BagImplConstructor
-                        _ _  DelegateReps DelegateImpls ValidImpls idx BagEmpty d).
-    intros; destruct idx as [idx [n nth_n]].
-    destruct n; simpl in *.
-    + unfold i2th_Bounded, ith_Bounded_rect; simpl.
-      destruct (H0 ()) as [r_o' [refines_r_o' AbsR_r_o']].
+                        _ _  _ DelegateReps DelegateImpls ValidImpls idx BagEmpty d).
+    revert qschemaSchemas IHqschemaSchemas DelegateReps idx' Index' DelegateImpls ValidImpls
+           v0 H H' H0.
+    pattern n, idx; apply Fin.caseS; simpl; intros.
+    + destruct (H0 ()) as [r_o' [refines_r_o' AbsR_r_o']].
       pose proof (refines_r_o' _ (ReturnComputes _)).
       unfold CallBagConstructor in H1; simpl in H1;  computes_to_inv; subst.
-      revert AbsR_r_o'; clear.
-      unfold Dep_Type_BoundedIndex_nth_eq, eq_rect_r, eq_rect, eq_sym.
-      pose eq_proofs_unicity.
-      injection nth_n; intros; subst.
-      match goal with
-          |- context [indexb_ibound_eq ?a ?a' ?eq'] =>
-          pose a; pose a'; pose eq'
-      end.
-      pose proof (fun H => eq_proofs_unicity H (indexb_ibound_eq b b0 e0) eq_refl).
-      revert H; unfold b, b0, e0; intros.
-      rewrite H.
-      revert AbsR_r_o'; clear.
-      match goal with
-          |- context [eq_proofs_unicity_Opt_A ?string_dec ?nth_n ?nth_n'] =>
-          destruct (eq_proofs_unicity_Opt_A string_dec nth_n nth_n');
-            rewrite (@eq_proof_unicity_eq _ string_dec ((relName a) :: map relName qschemaSchemas) (relName a) 0 nth_n nth_n eq_refl); eauto
-      end.
-      intros; destruct (string_dec x y); intuition.
-    + apply (H' {| bindex := idx;
-                  indexb := {| ibound := n;
-                               boundi := nth_n |} |}).
+      apply AbsR_r_o'.
+    + eapply H'.
 Qed.
 
 Definition Update_Build_IndexedQueryStructure_Impl_cRep
            qs_schema Index DelegateReps
-           (r_n : Build_IndexedQueryStructure_Impl_cRep (indices := qs_schema) Index DelegateReps)
+           (r_n : Build_IndexedQueryStructure_Impl_cRep (indices := qschemaSchemas qs_schema) Index DelegateReps)
            TableID (r_n' : DelegateReps TableID)
-: Build_IndexedQueryStructure_Impl_cRep Index DelegateReps :=
+: Build_IndexedQueryStructure_Impl_cRep Index DelegateReps.
+Admitted.
+(*  :=
   match TableID return DelegateReps TableID -> _ with
       {|bindex := idx;
         indexb := {| ibound := n;
                      boundi := nth_n |} |} =>
       Update_Iterate_Dep_Type string_dec DelegateReps r_n n nth_n
-  end r_n'.
+  end r_n'. *)
 
 Lemma Update_Build_IndexedQueryStructure_Impl_AbsR
 : forall qs_schema Index DelegateReps DelegateImpls
@@ -357,10 +333,11 @@ Lemma Update_Build_IndexedQueryStructure_Impl_AbsR
     -> AbsR (ValidImpls TableID) r_o' r_n'
     -> @Build_IndexedQueryStructure_Impl_AbsR
          qs_schema Index DelegateReps DelegateImpls
-         ValidImpls (UpdateIndexedRelation r_o TableID r_o')
-         (Update_Build_IndexedQueryStructure_Impl_cRep _ _ r_n TableID r_n').
+         ValidImpls (UpdateIndexedRelation _ _ r_o TableID r_o')
+         (Update_Build_IndexedQueryStructure_Impl_cRep _ _ _ r_n TableID r_n').
 Proof.
-  unfold Build_IndexedQueryStructure_Impl_AbsR,
+Admitted.
+(*  unfold Build_IndexedQueryStructure_Impl_AbsR,
   Update_Build_IndexedQueryStructure_Impl_cRep; intros.
   destruct (BoundedString_eq_dec TableID idx); subst.
   - destruct idx as [idx [n nth_n]]; simpl.
@@ -376,7 +353,7 @@ Proof.
     clear r_o' r_n' H0.
     unfold not; intros; subst; eapply n.
     apply idx_ibound_eq; simpl; eauto using string_dec.
-Qed.
+Qed. *)
 
 
 Arguments BuildIndexSearchTerm : simpl never.
@@ -683,9 +660,9 @@ Ltac convert_Where_to_filter :=
 
 Ltac equate X Y := let H := fresh in assert (H : X = Y) by reflexivity; clear H.
 
-Definition unit_Heading := BuildHeading [].
+Definition unit_Heading : RawHeading := {| AttrList := Vector.nil _ |}.
 
-Definition unit_Tuple : @Tuple unit_Heading := BuildTuple (inil _).
+Definition unit_Tuple : @RawTuple unit_Heading := inil2.
 
 Ltac get_ithDefault f n k :=
   match type of f with
@@ -695,8 +672,8 @@ Ltac get_ithDefault f n k :=
       let H := fresh "H" in
       let proj := fresh "proj" in
       let proj := eval simpl in
-      (fun b : ilist (@Tuple) A => ith_default unit_Heading unit_Tuple b n) in
-          evar (G : @Tuple (nth_default unit_Heading A n) -> C);
+      (fun b : ilist2 (@RawTuple) A => ith2 unit_Tuple b n) in
+          evar (G : @RawTuple (nth_default unit_Heading A n) -> C);
         assert (H : forall p,
                       f p = G (proj p)) by
           (subst G; intro p;
@@ -710,18 +687,18 @@ Ltac get_ithDefault f n k :=
 
 Ltac get_ithDefault_pair f m n k :=
   match type of f with
-    | ilist (@Tuple) ?A -> ?C =>
+    | ilist (@RawTuple) ?A -> ?C =>
       let G := fresh "G" in
       let p := fresh "p" in
       let H := fresh "H" in
       let proj1 := fresh "proj" in
       let proj2 := fresh "proj" in
       let proj1 := eval simpl in
-      (fun b : ilist (@Tuple) A => ith_default unit_Heading unit_Tuple b m) in
+      (fun b : ilist2 (B := @RawTuple) A => ith2 unit_Tuple b m) in
           let proj2 := eval simpl in
-          (fun b : ilist (@Tuple) A => ith_default unit_Heading unit_Tuple b n)
-            in evar (G : @Tuple (nth_default unit_Heading A m)
-                         -> @Tuple (nth_default unit_Heading A n)
+          (fun b : ilist (@RawTuple) A => ith2 unit_Tuple b n)
+            in evar (G : @RawTuple (nth_default unit_Heading A m)
+                         -> @RawTuple (nth_default unit_Heading A n)
                          -> C);
             assert (H : forall p,
                           f p = G (proj1 p) (proj2 p)) by
@@ -798,7 +775,7 @@ Ltac findGoodTerm_dep SC F indexed_attrs visited_attrs makeClause k :=
               | right _ => k (fd :: visited_attrs)
                              ({| KindNameKind := EqualityIndex;
                                  KindNameName := fd|}, X)
-                             (fun (a : T) (_ : @Tuple SC) => true)
+                             (fun (a : T) (_ : @RawTuple SC) => true)
               | left _ => k visited_attrs tt F
             end
         | forall a b, {GetAttribute _ ?fd' = @?X a} + {_} =>
@@ -812,7 +789,7 @@ Ltac findGoodTerm_dep SC F indexed_attrs visited_attrs makeClause k :=
             | right _ => k (fd :: visited_attrs)
                            ({| KindNameKind := EqualityIndex;
                                KindNameName := fd|}, X)
-                           (fun (a : T) (_ : @Tuple SC) => true)
+                           (fun (a : T) (_ : @RawTuple SC) => true)
               | left _ => k visited_attrs tt F
             end
 
@@ -826,14 +803,14 @@ Ltac findGoodTerm_dep SC F indexed_attrs visited_attrs makeClause k :=
                 findGoodTerm_dep
                   SC g indexed_attrs v makeClause
                   ltac:(fun v' fds2 tail2 =>
-                          k v' (fds1, fds2) (fun (a : T) (tup : @Tuple SC) =>
+                          k v' (fds1, fds2) (fun (a : T) (tup : @RawTuple SC) =>
                                                (tail1 a tup) && (tail2 a tup))))
     | _ => k visited_attrs tt F
   end.
 
 Definition Dep_SearchTerm_Wrapper {A} {heading}
-           (search_term_dep : @Tuple heading -> A)
-           (tup : @Tuple heading) : A := search_term_dep tup.
+           (search_term_dep : @RawTuple heading -> A)
+           (tup : @RawTuple heading) : A := search_term_dep tup.
 
 Ltac find_simple_search_term_dep
      makeClause EarlyIndex LastIndex
@@ -879,11 +856,11 @@ Ltac find_equivalent_search_term_pair build_search_term_dep :=
       [ H : @DelegateToBag_AbsR ?qs_schema ?indices ?r_o ?r_n
         |- ExtensionalEq ?f _ ] =>
       match type of f with
-        | ilist (@Tuple) (?heading :: ?headings) -> bool =>
-          makeEvar (ilist (@Tuple) headings -> @Tuple heading -> bool)
+        | ilist (@RawTuple) (?heading :: ?headings) -> bool =>
+          makeEvar (ilist (@RawTuple) headings -> @RawTuple heading -> bool)
                    ltac:(fun filter_dec =>
                            let eqv_f_dec := fresh in
-                           assert (forall a : ilist (@Tuple) (heading :: headings),
+                           assert (forall a : ilist (@RawTuple) (heading :: headings),
                                      f a = filter_dec (ilist_tl a) (ilist_hd a));
                          [let a := fresh in
                           intro a; let f' := match goal with |- ?f = _ => f end in
@@ -892,7 +869,7 @@ Ltac find_equivalent_search_term_pair build_search_term_dep :=
                                        with | ?f'' _ _ => f'' end
                                          in let f3 := eval simpl in f'' in
                                                 unify f3 filter_dec; reflexivity
-                                       | let dom := constr:(ilist (@Tuple) headings) in
+                                       | let dom := constr:(ilist (@RawTuple) headings) in
                                          let schemas := eval simpl in (qschemaSchemas qs_schema) in
                                              find_equivalent_tuple schemas heading
                                                                    ltac:(fun id => let idx' := constr:({| bindex := id |} : BoundedIndex (map relName (qschemaSchemas qs_schema)))
@@ -904,14 +881,14 @@ Ltac find_equivalent_search_term_pair build_search_term_dep :=
                                                                                                           makeEvar (dom -> search_term_type)
                                                                                                                ltac: (fun search_term =>
                                                                                                                         let eqv := fresh in
-                                                                                                                        assert (forall (a : ilist (@Tuple) (headings)) (b : @Tuple heading) ,
+                                                                                                                        assert (forall (a : ilist (@RawTuple) (headings)) (b : @RawTuple heading) ,
                                                                                                                                   filter_dec a b = search_term_matcher (search_term a) b) as eqv;
                                                                                                                       [ build_search_term_dep qs_schema idx dom filter_dec search_term
                                                                                                                       | match goal with
                                                                                                                             |- ExtensionalEq ?f ?search_term' =>
                                                                                                                             match type of f with
-                                                                                                                              | ilist (@Tuple) (?A :: ?As) -> _ =>
-                                                                                                                                unify search_term' (fun a : ilist (@Tuple) (A :: As) => search_term_matcher (search_term (ilist_tl a)) (ilist_hd a))
+                                                                                                                              | ilist (@RawTuple) (?A :: ?As) -> _ =>
+                                                                                                                                unify search_term' (fun a : ilist (@RawTuple) (A :: As) => search_term_matcher (search_term (ilist_tl a)) (ilist_hd a))
                                                                                                                             end
                                                                                                                         end;
                                                                                                                         unfold ExtensionalEq in *;
@@ -929,7 +906,7 @@ Ltac find_equivalent_search_term build_search_term :=
       get_ithDefault f 0
                      ltac:(fun filter_dec =>
                              let heading := match type of filter_dec with
-                                              | @Tuple ?heading -> bool => constr:(heading)
+                                              | @RawTuple ?heading -> bool => constr:(heading)
                                             end in
                              let schemas := eval simpl in (qschemaSchemas qs_schema) in
                                  find_equivalent_tuple schemas heading
@@ -950,7 +927,7 @@ Ltac find_equivalent_search_term build_search_term :=
                                                                                                                 |- ExtensionalEq ?f ?search_term' =>
                                                                                                                 match type of f with
                                                                                                                   | ?A -> _ =>
-                                                                                                                    unify search_term' (fun a : A => search_term_matcher search_term (ith_default unit_Heading unit_Tuple a 0))
+                                                                                                                    unify search_term' (fun a : A => search_term_matcher search_term (ith2 unit_Tuple a 0))
                                                                                                                 end
                                                                                                             end;
                                                                                                             unfold ExtensionalEq in *; intros;
@@ -998,7 +975,7 @@ Ltac convert_filter_to_find' :=
     | H : @DelegateToBag_AbsR ?qs_schema ?indices ?r_o ?r_n
       |- context[l <- CallBagMethod ?idx BagFind ?r_n ?st;
                   l' <- Join_Comp_Lists (Build_single_Tuple_list (snd l))
-                     (fun _ : ilist (@Tuple) [?heading] =>
+                     (fun _ : ilist (@RawTuple) [?heading] =>
                         l <- CallBagMethod ?idx' BagEnumerate ?r_n ();
                       ret (snd l));
                   List_Query_In (filter (fun a => @?f a && @?filter_rest a) l') ?resultComp] =>
@@ -1054,15 +1031,15 @@ Ltac ilist_of_dep_evar C D B As k :=
   end.
 
 Definition Join_Comp_Lists'
-           {A : Type} {f : A -> Type} {As : list A} {a : A}
-           (l : list (ilist f As)) (c : ilist f As -> list (f a))
+           {n} {A : Type} {f : A -> Type} {As : Vector.t A n} {a : A}
+           (l : list (ilist2 (B := f) As)) (c : ilist2 (B := f) As -> list (f a))
   := flatten (map
-                (fun l' => map (fun fa : f a => icons _ fa l') (c l')) l).
+                (fun l' => map (fun fa : f a => icons2 fa l') (c l')) l).
 
-Lemma Join_Comp_Lists_Impl {A : Type} {f : A -> Type} {As : list A} {a : A}
-: forall (l : list (ilist f As))
-         (c : ilist f As -> Comp (list (f a)))
-         (c' : ilist f As -> list (f a)),
+Lemma Join_Comp_Lists_Impl {n} {A : Type} {f : A -> Type} {As : Vector.t A n} {a : A}
+: forall (l : list (ilist2 (B := f) As))
+         (c : ilist2 As -> Comp (list (f a)))
+         (c' : ilist2 As -> list (f a)),
     (forall a', refine (c a') (ret (c' a')))
     -> refine (Join_Comp_Lists l c) (ret (Join_Comp_Lists' l c')).
 Proof.
@@ -1073,9 +1050,6 @@ Proof.
     reflexivity.
 Qed.
 
-Arguments icons {A} {B} {a} {As} _ _.
-Arguments CallBagConstructor {heading} name {index} cidx _ _.
-
 Ltac implement_bag_constructors :=
   repeat match goal with
            | |- context[ Pick (fun r_n : @Build_IndexedQueryStructure_Impl_cRep ?qs_schema ?Index ?DelegateReps =>
@@ -1085,7 +1059,7 @@ Ltac implement_bag_constructors :=
              refine pick val (@Initialize_IndexedQueryStructureImpls' qs_schema Index DelegateReps DelegateImpls);
                [ higher_order_reflexivity |
                  unfold Build_IndexedQueryStructure_Impl_AbsR;
-                   eapply Iterate_Dep_Type_BoundedIndex_equiv_1; simpl; intuition ]
+                   eapply Lookup_Iterate_Dep_Type; simpl; intuition ]
            | |- context[CallBagConstructor ?ridx ?cidx ?d] =>
              match goal with
                  |- appcontext[@Build_IndexedQueryStructure_Impl_AbsR
@@ -1293,8 +1267,8 @@ Ltac implement_Insert_branches :=
            end
   ].
 
-Ltac remove_spurious_Dep_Type_BoundedIndex_nth_eq :=
-  match goal with
+Ltac remove_spurious_Dep_Type_BoundedIndex_nth_eq := idtac.
+(*  match goal with
     | |- context[Dep_Type_BoundedIndex_nth_eq ?A_eq_dec (As := ?As) ?P ?n ?nth ?nth ?p] =>
       rewrite (@Dep_Type_BoundedIndex_nth_eq_refl _ A_eq_dec As P _ n nth p)
     (* Handle the case when the two equalities are eq_refl, but one use the Specif.value
@@ -1305,7 +1279,7 @@ Ltac remove_spurious_Dep_Type_BoundedIndex_nth_eq :=
         | |- context[Dep_Type_BoundedIndex_nth_eq ?A_eq_dec (As := As) ?P ?n ?nth ?nth ?p] =>
           rewrite (@Dep_Type_BoundedIndex_nth_eq_refl _ A_eq_dec As P _ n nth p)
       end
-  end.
+  end. *)
 
 Lemma Implement_Bound_Bag_Call' A
 : forall qs_schema Index DelegateReps DelegateImpls ValidImpls
@@ -1648,13 +1622,13 @@ Ltac distribute_filters_to_joins' :=
                                         (filter (fun a : ilist _ (?heading1 :: ?heading2 :: ?headings) =>
                                                    @?f a && @?g a) l') ?l2' ?cond2)
                                      _ => first (* No test case for this branch *)
-                                            [ makeEvar (ilist (@Tuple) headings -> bool)
+                                            [ makeEvar (ilist (@RawTuple) headings -> bool)
                                                        ltac:(fun f' =>
                                                                find_equiv_tl heading1 headings f f';
                                                              let Comp_l2 := fresh in
                                                              assert
-                                                               (forall a : ilist (@Tuple) headings,
-                                                                exists v : list (@Tuple heading1),
+                                                               (forall a : ilist (@RawTuple) headings,
+                                                                exists v : list (@RawTuple heading1),
                                                                   refine (l2 a) (ret v)) as Comp_l2
                                                                  by Realize_CallBagMethods;
                                                              etransitivity;
@@ -1667,13 +1641,13 @@ Ltac distribute_filters_to_joins' :=
                                       Join_Filtered_Comp_Lists (a := ?heading2)
                                                                (@filter (ilist _ (?heading1 :: ?headings)) ?f l') ?l2' ?cond2) _
                            =>   first
-                                  [ makeEvar (ilist (@Tuple) headings -> bool) (* No test case for this branch either *)
+                                  [ makeEvar (ilist (@RawTuple) headings -> bool) (* No test case for this branch either *)
                                              ltac:(fun f' =>
                                                      find_equiv_tl heading1 headings f f';
                                                    let Comp_l2 := fresh in
                                                    assert
-                                                     (forall a : ilist (@Tuple) headings,
-                                                      exists v : list (@Tuple heading1),
+                                                     (forall a : ilist (@RawTuple) headings,
+                                                      exists v : list (@RawTuple heading1),
                                                         refine (l2 a) (ret v)) as Comp_l2
                                                        by Realize_CallBagMethods;
                                                    etransitivity;
@@ -1697,12 +1671,12 @@ Ltac distribute_filters_to_joins' :=
                                                   (filter (fun a : ilist _ (?heading :: ?headings) =>
                                                              @?f a && @?g a) l') ?resultComp)
                                    _ =>
-                         first [makeEvar (ilist (@Tuple) headings -> bool)
+                         first [makeEvar (ilist (@RawTuple) headings -> bool)
                                          ltac:(fun f' => find_equiv_tl heading headings f f';
                                                let Comp_l2 := fresh in
                                                assert
-                                                 (forall a : ilist (@Tuple) headings,
-                                                  exists v : list (@Tuple heading),
+                                                 (forall a : ilist (@RawTuple) headings,
+                                                  exists v : list (@RawTuple heading),
                                                     refine (l2 a) (ret v)) as Comp_l2
                                                    by Realize_CallBagMethods;
                                                etransitivity;
@@ -1716,12 +1690,12 @@ Ltac distribute_filters_to_joins' :=
                                List_Query_In (ResultT := ?ResultT)
                                              (@filter (ilist _ (?heading :: ?headings)) ?f l') ?resultComp)
                               _ =>
-                         first [ makeEvar (ilist (@Tuple) headings -> bool)
+                         first [ makeEvar (ilist (@RawTuple) headings -> bool)
                                           ltac:(fun f' => find_equiv_tl heading headings f f';
                                                 let Comp_l2 := fresh in
                                                 assert
-                                                  (forall a : ilist (@Tuple) headings,
-                                                   exists v : list (@Tuple heading),
+                                                  (forall a : ilist (@RawTuple) headings,
+                                                   exists v : list (@RawTuple heading),
                                                      refine (l2 a) (ret v)) as Comp_l2 by
                                                       Realize_CallBagMethods;
                                                 apply (@refine_Join_Filtered_Comp_Lists_filter_hd heading headings f' ResultT resultComp l2 Comp_l2 l1))
@@ -1759,7 +1733,7 @@ Ltac convert_filter_search_term_to_find :=
         | fun a => (?MatchIndexSearchTerm (@?st a) (ilist_hd a)) && true =>
           let stT := type of st in
           match stT with _ -> ?stT =>
-                         makeEvar (ilist (@Tuple) headings -> stT)
+                         makeEvar (ilist (@RawTuple) headings -> stT)
                                   ltac:(fun st_dep =>
                                           let eqv := fresh in
                                           let a := fresh in
@@ -1997,7 +1971,7 @@ Ltac plan CreateTerm EarlyIndex LastIndex
                makeClause_dep EarlyIndex_dep LastIndex_dep
   end.
 
-Ltac master_plan' matchIndex
+(*Ltac master_plan' matchIndex
      CreateTerm EarlyIndex LastIndex
      makeClause_dep EarlyIndex_dep LastIndex_dep :=
   (* Implement constraints as queries. *)
@@ -2033,7 +2007,7 @@ Ltac partial_master_plan' matchIndex
               plan CreateTerm EarlyIndex LastIndex
                    makeClause_dep EarlyIndex_dep LastIndex_dep
           end
-         ).
+         ). *)
 
 Ltac matchEqIndex WhereClause k := fail.
 Ltac EqIndexUse SC F indexed_attrs f k := fail.
@@ -2049,11 +2023,11 @@ Ltac EqIndexTactics f :=
     EqIndexUse_dep createEarlyEqualityTerm_dep createLastEqualityTerm_dep
     f.
 
-Ltac master_plan IndexTactics := IndexTactics master_plan'.
+(* Ltac master_plan IndexTactics := IndexTactics master_plan'.
 Ltac partial_master_plan IndexTactics := IndexTactics partial_master_plan'.
 
 Ltac simple_master_plan := master_plan EqIndexTactics.
-Ltac simple_partial_master_plan := partial_master_plan EqIndexTactics.
+Ltac simple_partial_master_plan := partial_master_plan EqIndexTactics. *)
 
 Global Opaque CallBagMethod.
 Global Opaque CallBagConstructor.
