src/QueryStructure/Automation/Constraints/FunctionalDependencyAutomation.v
@@ -1,5 +1,10 @@
-Require Export Fiat.QueryStructure.Specification.Representation.QueryStructureNotations Fiat.QueryStructure.Specification.Operations.Query.
-Require Import Coq.Lists.List Coq.Arith.Compare_dec Coq.Bool.Bool Coq.Strings.String Coq.Strings.Ascii
+Require Export Fiat.QueryStructure.Specification.Representation.QueryStructureNotations
+        Fiat.QueryStructure.Specification.Operations.Query.
+Require Import Coq.Lists.List
+        Coq.Arith.Compare_dec
+        Coq.Bool.Bool
+        Coq.Strings.String
+        Coq.Strings.Ascii
         Fiat.Common.BoolFacts
         Fiat.Common.List.PermutationFacts
         Fiat.Common.List.ListMorphisms
