src/QueryStructure/Specification/Representation/QueryStructureNotations.v
@@ -39,9 +39,9 @@ Open Scope QuerySpec.
 Open Scope string_scope.
 Open Scope Tuple.
 Open Scope comp_scope.
-
+(* Notation Test. *)
 (* Let's define some synonyms for strings we'll need,
- * to save on type-checking time. *)
+ * to save on type-checking time.
 Definition sBOOKS := "Books".
 Definition sAUTHOR := "Authors".
 Definition sTITLE := "Title".
@@ -88,9 +88,11 @@ Definition BookStoreSig : ADTSig :=
       Method "NumOrders" : rep x string -> rep x nat
     }.
 
+Print QSDelete.
+Print QSInsert.
 (* Now we write what the methods should actually do. *)
 
-(*Definition BookStoreSpec : ADT BookStoreSig.
+Definition BookStoreSpec : ADT BookStoreSig.
   refine ( QueryADTRep BookStoreSchema {
     Def Constructor "Init" (_ : unit) : rep := empty,
 
@@ -118,9 +120,13 @@ Definition BookStoreSig : ADTSig :=
                  Return ())
 } ).
 
-  Check QSDelete.
-  let b := constr:(@qsSchemaHint' _H0 : QueryStructureSchema) in 
-  unify (b) (BookStoreSchema). 
+  pose (Delete o from sORDERS where True).
+  Set Printing All.
+  idtac.
+  simpl in c.
+  apply c.
+  let b := constr:(@qsSchemaHint' _H0 : QueryStructureSchema) in
+  unify (b) (BookStoreSchema).
   (* match goal with
     |- ?A =>
     match type of (Delete o from sORDERS where True : A) with
